Introduce non-atomic invariants

nola/examples/logic/iris.v
@@ -1,15 +1,42 @@
 (** * Iris preliminaries *)
 
 From nola.examples.logic Require Export prop.
-From nola Require Export sintp iris.inv iris.wp.
+From nola Require Export sintp.
+From nola.iris Require Export inv na_inv wp.
 From nola.examples.heap_lang Require Export primitive_laws.
 
-(** ** [nintpGS]: Iris resources *)
+(** ** Iris resources *)
 
+(** Data for invariant *)
+Variant nid : Type :=
+| (* usual *) nid_u : nPropS (;ᵞ) → nid
+| (* non-atomic *) nid_na : na_inv_pool_name → positive → nPropS (;ᵞ) → nid.
+
+(** [nintpGS]: Iris resource *)
 Class nintpGS (Σ : gFunctors) := NintpG {
   nintpGS_heapGS :: heapGS_gen HasNoLc Σ;
-  nintpGS_ninvGS :: ninvGS (nPropS (;ᵞ)) Σ;
+  nintpGS_ninvGS :: ninvGS nid Σ;
+  nintpGS_na_invG :: na_invG Σ;
 }.
+
+Section nid_intp.
+  Context `{!nintpGS Σ}.
+
+  (** Interpret [nid] *)
+  Definition nid_intp (intp : nPropS (;ᵞ) -d> iProp Σ) : nid -d> iProp Σ :=
+    λ Px, match Px with
+    | nid_u P => intp P
+    | nid_na p i P => na_body p i (intp P)
+    end.
+  #[export] Instance nid_intp_ne : NonExpansive nid_intp.
+  Proof. solve_proper. Qed.
+
+  (** [ninv_wsat] for [nid] *)
+  Definition ninv_wsat' (intp : nPropS (;ᵞ) -d> iProp Σ) : iProp Σ :=
+    ninv_wsat (nid_intp intp).
+  #[export] Instance ninv_wsat'_ne : NonExpansive ninv_wsat'.
+  Proof. solve_proper. Qed.
+End nid_intp.
 
 (** ** For strong interpretation *)
 
@@ -35,4 +62,18 @@ Section iris.
   Lemma nninv_unseal : nninv = nninv_def. Proof. exact nninv_aux.(seal_eq). Qed.
   #[export] Instance nninv_persistent {s i N P} : Persistent (nninv s i N P).
   Proof. rewrite nninv_unseal. apply _. Qed.
+
+  (** ** [na_nninv]: Non-atomic [ninv] in the accessor style *)
+  Definition na_nninv_def (s : nsintp_ty Σ) (i : nat)
+    (p : na_inv_pool_name) (N : namespace) (P : nPropL (;ᵞ)) : iProp Σ :=
+    □ ⸨ ∀ E F, ⌜↑N ⊆ E⌝ → ⌜↑N ⊆ F⌝ → n_na_own p F =[n_inv_wsat]{E,E∖↑N}=∗
+          P ∗ n_na_own p (F∖↑N) ∗
+          (P -∗ n_na_own p (F∖↑N) =[n_inv_wsat]{E∖↑N,E}=∗ n_na_own p F) ⸩(s, i).
+  Definition na_nninv_aux : seal na_nninv_def. Proof. by eexists. Qed.
+  Definition na_nninv := na_nninv_aux.(unseal).
+  Lemma na_nninv_unseal : na_nninv = na_nninv_def.
+  Proof. exact na_nninv_aux.(seal_eq). Qed.
+  #[export] Instance na_nninv_persistent {s i p N P} :
+    Persistent (na_nninv s i p N P).
+  Proof. rewrite na_nninv_unseal. apply _. Qed.
 End iris.
