nola/iris/na_inv.v
@@ -1,0 +1,50 @@
+(** * For non-atomic invariants *)
+
+From nola Require Export iris.inv.
+From iris.base_logic Require Export lib.na_invariants.
+From iris.algebra Require Import gset coPset.
+From iris.proofmode Require Import proofmode.
+
+Section na_ninv.
+  Context `{!invGS_gen hlc Σ, !na_invG Σ}.
+  Local Existing Instance na_inv_inG.
+
+  (** Access lock of an non-atomic invariant *)
+  Definition na_lock (p : na_inv_pool_name) (i : positive) : iProp Σ :=
+    own p (ε, GSet {[i]}).
+
+  (** What to be put in an non-atomic invariant *)
+  Definition na_body
+    (p : na_inv_pool_name) (i : positive) (P : iProp Σ) : iProp Σ :=
+    P ∗ na_lock p i ∨ na_own p {[i]}.
+  #[export] Instance na_body_ne {p i} : NonExpansive (na_body p i).
+  Proof. solve_proper. Qed.
+
+  (** Allocate [na_lock] *)
+  Lemma na_lock_alloc {p N} :
+    ⊢ |==> ∃ i, ⌜i ∈ (↑N:coPset)⌝ ∧ na_lock p i.
+  Proof.
+    iMod (own_unit (prodUR coPset_disjUR (gset_disjUR positive)) p) as "ε".
+    iMod (own_updateP with "ε") as ([m1 m2]) "[%cond lock]".
+    { apply prod_updateP'.
+      - apply cmra_updateP_id, (reflexivity (R:=eq)).
+      - apply (gset_disj_alloc_empty_updateP_strong' (.∈ (↑N:coPset)))=> ?.
+        apply fresh_inv_name. }
+    move: cond=>/=[<-[i[->?]]]. iModIntro. iExists i. by iSplit.
+  Qed.
+
+  (** Access [P] from [na_body] *)
+  Lemma na_body_acc {p i N E P} :
+    i ∈ (↑N:coPset) → ↑N ⊆ E →
+    na_body p i P -∗ na_own p E -∗ P ∗ na_own p (E∖↑N) ∗
+      (P -∗ na_own p (E∖↑N) -∗ na_body p i P ∗ na_own p E).
+  Proof.
+    iIntros (??) "[[$ lock]|i] E"; last first.
+    { iDestruct (na_own_disjoint with "i E") as %?. set_solver. }
+    rewrite [E as X in na_own p X](union_difference_L (↑N) E); [|done].
+    rewrite [X in (X ∪ _)](union_difference_L {[i]} (↑N)) ?na_own_union;
+      [|set_solver..].
+    iDestruct "E" as "[[i $] $]". iIntros "P $". iSplitR "i"; [|done].
+    iLeft. iFrame.
+  Qed.
+End na_ninv.
